\documentclass{article}
\usepackage{epsfig}
\pagestyle{empty}
\begin{document}
\[ Bin_i=\Sum_j\neqi Bin_j \]
\pagebreak

$\frac{1}{h}\tan^{-1}{\frac{Qh_X}{Qh_Y}}$
\pagebreak

$ Qn = \frac{Qn}{M} $
\pagebreak

$ Qn = \frac{Qn}{\sqrt{M}} $
\pagebreak

\[ Q' = \mathcal{R}(\Delta \phi) Q \]
\pagebreak

$ \Delta \phi $
\pagebreak

\[ \Delta \phi_n = - \frac{1}{m} \tan^{-1} \left(\frac{\langle{Q_n}_X{Q^A_m}_Y\rangle - \langle{Q_n}_Y{Q^A_m}_X\rangle} {\langle{Q_n}_X{Q^A_m}_X\rangle + \langle{Q_n}_Y{Q^A_m}_Y\rangle}\right) \]
\pagebreak

$ \langle \cdots \rangle $
\pagebreak

$ A $
\pagebreak

$ m $
\pagebreak

\[ \frac{\Sigma \mbox{fValues(bin)}}{\mbox{fEntries(bin)}} \]
\pagebreak

\[ \sqrt{\frac{\Sigma \mbox{fValues}^2\mbox{(bin)}}{\mbox{fEntries(bin)}} - \left(\frac{\Sigma \mbox{fValues(bin)}}{\mbox{fEntries(bin)}}\right)^2} \]
\pagebreak

\[ \frac{\sqrt{\frac{\Sigma \mbox{fValues}^2\mbox{(bin)}}{\mbox{fEntries(bin)}} - \left(\frac{\Sigma \mbox{fValues(bin)}}{\mbox{fEntries(bin)}}\right)^2}} {\sqrt{\mbox{fEntries(bin)}}} \]
\pagebreak

$ \mbox{Q'} = \mbox{Q}$
\pagebreak

$ \mbox{Q'} = \frac{\mbox{Q}}{\sqrt{\mbox{M}}} $
\pagebreak

$ \mbox{Q'} = \frac{\mbox{Q}}{\mbox{M}} $
\pagebreak

$ \mbox{Q'} = \frac{\mbox{Q}}{|\mbox{Q}|} $
\pagebreak

$ \mbox{M}_{c,i} $
\pagebreak

$ c $
\pagebreak

$ i $
\pagebreak

\[ \mbox{M}'_{c,i} = \frac{\mbox{M}_{c,i}}{\langle\mbox{M}_{c}\rangle} \]
\pagebreak

$\langle\mbox{M}_{c}\rangle$
\pagebreak

\[ \langle\mbox{M}_{c}\rangle = \frac{1}{\mbox{N}_{ev}} \Sigma_{i}^{\mbox{N}_{ev}} \mbox{M}_{c,i} \]
\pagebreak

\[ \mbox{M}'_{c,i} = \mbox{A} + \mbox{B} \frac{\mbox{M}_{c,i} - \langle\mbox{M}_{c}\rangle} {\sigma_{{M}_{c}}} \]
\pagebreak

$\sigma_{{M}_{c}}$
\pagebreak

$c$
\pagebreak

\[ \sigma_{{M}_{c}} = \sqrt{ \frac{1}{\mbox{N}_{ev}} \Sigma_{i}^{\mbox{N}_{ev}} \mbox{M}^2_{c,i} - \frac{1}{\mbox{N}^2_{ev}} \left(\Sigma_{i}^{\mbox{N}_{ev}} \mbox{M}_{c,i}\right)^2} \]
\pagebreak

$ \mbox{M'} = \mbox{M}$
\pagebreak

$ \mbox{M}' = \frac{\mbox{M}}{\langle\mbox{M}\rangle} $
\pagebreak

$ \mbox{M}' = \mbox{A} + \mbox{B} \frac{\mbox{M} - \langle\mbox{M} \rangle}{\sigma_{{M}}} $
\pagebreak

\[ Q' = Q - {\langle Q \rangle} \]
\pagebreak

$\langle Q \rangle$
\pagebreak

\[ \langle Q \rangle = \frac{1}{\mbox{N}_{ev}} \sum_{i}^{\mbox{N}_{ev}} Q_i \]
\pagebreak

\[ Q' = \frac{Q- \langle Q \rangle}{\sigma_Q} \]
\pagebreak

$ \sigma_Q $
\pagebreak

$ Q $
\pagebreak

\[ \sigma_Q = \sqrt{ \frac{1}{\mbox{N}_{ev}} \sum_{i}^{\mbox{N}_{ev}} Q^2_i - \frac{1}{\mbox{N}^2_{ev}} \left(\sum_{i}^{\mbox{N}_{ev}} Q_i \right)^2} \]
\pagebreak

\[ Q_{n,(x,y)}' = \frac{Q_{n,(x,y)} - \Lambda^{s(-,+)}_{2n} Q_{n,(y,x)}}{1 - \Lambda^{s-}_{2n}\Lambda^{s+}_{2n}} \]
\pagebreak

\[ Q''_{n(x,y)} = \frac{Q'_{n(x,y)}}{A_{2n}^{(+,-)}} \]
\pagebreak

$ A_{2n}^{(+,-)} $
\pagebreak

$ \Lambda^{s(+,-)}_{2n} $
\pagebreak

\[ A^{\pm}_{2n} = 1 \pm \langle X_{2n} \rangle \]
\pagebreak

\[ \Lambda ^{\pm}_{2n} = \frac{\langle Y_{2n} \rangle}{A^{\pm}_{2n}} \]
\pagebreak

$ B $
\pagebreak

$ C $
\pagebreak

\[ A^{A+}_{2n} = \frac{\sqrt{2 \langle X^{A}_{n} X^{C}_{n} \rangle}\langle X^{A}_{n} X^{B}_{n} \rangle} {\sqrt{\langle X^{A}_{n} X^{B}_{n} \rangle \langle X^{B}_{n} X^{C}_{n} \rangle + \langle X^{A}_{n} Y^{B}_{n} \rangle \langle X^{B}_{n} Y^{C}_{n} \rangle}}, \]
\pagebreak

\[ A^{A-}_{2n} = \frac{\sqrt{2 \langle X^{A}_{n} X^{C}_{n} \rangle}\langle Y^{A}_{n} Y^{B}_{n} \rangle} {\sqrt{\langle X^{A}_{n} X^{B}_{n} \rangle \langle X^{B}_{n} X^{C}_{n} \rangle + \langle X^{A}_{n} Y^{B}_{n} \rangle \langle X^{B}_{n} Y^{C}_{n} \rangle}}, \]
\pagebreak

\[ \Lambda^{A,+}_{2n} = \frac{\langle X^{A}_{n} Y^{B}_{n} \rangle}{\langle X^{A}_{n} X^{B}_{n} \rangle} \]
\pagebreak

\[ \Lambda^{A,-}_{2n} = \frac{\langle X^{A}_{n} Y^{B}_{n} \rangle}{\langle Y^{A}_{n} Y^{B}_{n} \rangle} \]
\pagebreak

$ A^{\pm}_{2n} = 1 \pm \langle X_{2n} \rangle, \qquad \Lambda ^{\pm}_{2n} = \frac{\langle Y_{2n} \rangle}{A^{\pm}_{2n}} $
\pagebreak

$ A^{A+}_{2n} = \frac{\sqrt{2 \langle X^{A}_{n} X^{C}_{n} \rangle}\langle X^{A}_{n} X^{B}_{n} \rangle} {\sqrt{\langle X^{A}_{n} X^{B}_{n} \rangle \langle X^{B}_{n} X^{C}_{n} \rangle + \langle X^{A}_{n} Y^{B}_{n} \rangle \langle X^{B}_{n} Y^{C}_{n} \rangle}}, \\ \, A^{A-}_{2n} = \frac{\sqrt{2 \langle X^{A}_{n} X^{C}_{n} \rangle}\langle Y^{A}_{n} Y^{B}_{n} \rangle} {\sqrt{\langle X^{A}_{n} X^{B}_{n} \rangle \langle X^{B}_{n} X^{C}_{n} \rangle + \langle X^{A}_{n} Y^{B}_{n} \rangle \langle X^{B}_{n} Y^{C}_{n} \rangle}}, \\ \, \Lambda^{A,+}_{2n} = \frac{\langle X^{A}_{n} Y^{B}_{n} \rangle}{\langle X^{A}_{n} X^{B}_{n} \rangle}, \quad \Lambda^{A,-}_{2n} = \frac{\langle X^{A}_{n} Y^{B}_{n} \rangle}{\langle Y^{A}_{n} Y^{B}_{n} \rangle} $
\pagebreak

\end{document}
